_:AX2dX2fe0ec5fX3aX158de32f70eX3aXX2dX7ff8 <http://www.w3.org/2002/07/owl#onDataRange> <http://www.w3.org/2002/07/owl#rational> .
_:AX2dX2fe0ec5fX3aX158de32f70eX3aXX2dX7ff8 <http://www.w3.org/2002/07/owl#qualifiedCardinality> "1"^^<http://www.w3.org/2001/XMLSchema#nonNegativeInteger> .
_:AX2dX2fe0ec5fX3aX158de32f70eX3aXX2dX7ff8 <http://www.w3.org/2002/07/owl#onProperty> <http://w3id.org/abdn/socialmedia/prism#dataCollectionStarted> .
_:AX2dX2fe0ec5fX3aX158de32f70eX3aXX2dX7ff8 <http://www.w3.org/1999/02/22-rdf-syntax-ns#type> <http://www.w3.org/2002/07/owl#Restriction> .
<http://w3id.org/abdn/socialmedia/prism#dataCollectionStarted> <http://www.w3.org/2000/01/rdf-schema#comment> "The date that the activity of collected data started."@en .
<http://w3id.org/abdn/socialmedia/prism#dataCollectionStarted> <http://www.w3.org/2000/01/rdf-schema#label> "data Collection Started" .
<http://w3id.org/abdn/socialmedia/prism#dataCollectionStarted> <http://www.w3.org/2000/01/rdf-schema#range> <http://www.w3.org/2001/XMLSchema#date> .
<http://w3id.org/abdn/socialmedia/prism#dataCollectionStarted> <http://www.w3.org/1999/02/22-rdf-syntax-ns#type> <http://www.w3.org/2002/07/owl#DatatypeProperty> .
<http://w3id.org/abdn/socialmedia/prism#toNumber> <http://www.w3.org/2000/01/rdf-schema#comment> "Data preparation method in which the type of a datum is changed from text to number.   Based on transformation of the same label in OpenRefine."@en .
<http://w3id.org/abdn/socialmedia/prism#toNumber> <http://www.w3.org/2004/02/skos/core#prefLabel> "Convert text to number" .
<http://w3id.org/abdn/socialmedia/prism#toNumber> <http://www.w3.org/2000/01/rdf-schema#label> "Convert text to number" .
<http://w3id.org/abdn/socialmedia/prism#toNumber> <http://www.w3.org/1999/02/22-rdf-syntax-ns#type> <http://w3id.org/abdn/socialmedia/prism#DataPreparationMethod> .
_:AX2dX2fe0ec5fX3aX158de32f70eX3aXX2dX7ffb <http://www.w3.org/2002/07/owl#allValuesFrom> <http://w3id.org/abdn/socialmedia/prism#DataAnalysisMethod> .
_:AX2dX2fe0ec5fX3aX158de32f70eX3aXX2dX7ffb <http://www.w3.org/2002/07/owl#onProperty> <http://w3id.org/abdn/socialmedia/prism#analysisMethodUsed> .
_:AX2dX2fe0ec5fX3aX158de32f70eX3aXX2dX7ffb <http://www.w3.org/1999/02/22-rdf-syntax-ns#type> <http://www.w3.org/2002/07/owl#Restriction> .
<http://w3id.org/abdn/socialmedia/prism#textTransformation> <http://www.w3.org/2000/01/rdf-schema#comment> "Data preparation method in which text is transformed.   Based on transformation of the same name in OpenRefine."@en .
<http://w3id.org/abdn/socialmedia/prism#textTransformation> <http://www.w3.org/2004/02/skos/core#prefLabel> "Transform text" .
<http://w3id.org/abdn/socialmedia/prism#textTransformation> <http://www.w3.org/2000/01/rdf-schema#label> "Transform text" .
<http://w3id.org/abdn/socialmedia/prism#textTransformation> <http://www.w3.org/1999/02/22-rdf-syntax-ns#type> <http://w3id.org/abdn/socialmedia/prism#DataPreparationMethod> .
<http://w3id.org/abdn/socialmedia/prism#preparationMethodUsed> <http://www.w3.org/2000/01/rdf-schema#comment> "Relationship between a data preparation activity and the preparation method/technique used."@en .
<http://w3id.org/abdn/socialmedia/prism#preparationMethodUsed> <http://www.w3.org/2000/01/rdf-schema#label> "preparation Method Used" .
<http://w3id.org/abdn/socialmedia/prism#preparationMethodUsed> <http://www.w3.org/1999/02/22-rdf-syntax-ns#type> <http://www.w3.org/2002/07/owl#DatatypeProperty> .
_:AX2dX2fe0ec5fX3aX158de32f70eX3aXX2dX7ff7 <http://www.w3.org/2002/07/owl#allValuesFrom> <http://dbpedia.org/resource/dataset> .
_:AX2dX2fe0ec5fX3aX158de32f70eX3aXX2dX7ff7 <http://www.w3.org/2002/07/owl#onProperty> <http://www.w3.org/ns/prov#used> .
_:AX2dX2fe0ec5fX3aX158de32f70eX3aXX2dX7ff7 <http://www.w3.org/1999/02/22-rdf-syntax-ns#type> <http://www.w3.org/2002/07/owl#Restriction> .
<http://w3id.org/abdn/socialmedia/prism#DataCollectionTool> <http://www.w3.org/2000/01/rdf-schema#comment> "A (software) tool used to collect data."@en .
<http://w3id.org/abdn/socialmedia/prism#DataCollectionTool> <http://www.w3.org/2000/01/rdf-schema#label> "Data Collection Tool" .
<http://w3id.org/abdn/socialmedia/prism#DataCollectionTool> <http://www.w3.org/1999/02/22-rdf-syntax-ns#type> <http://www.w3.org/2002/07/owl#Class> .
<http://w3id.org/abdn/socialmedia/prism#toDate> <http://www.w3.org/2000/01/rdf-schema#comment> "Data preparation method in which the type of a datum is changed from text to date.   Based on transformation of the same label in OpenRefine."@en .
<http://w3id.org/abdn/socialmedia/prism#toDate> <http://www.w3.org/2004/02/skos/core#prefLabel> "Convert text to  date" .
<http://w3id.org/abdn/socialmedia/prism#toDate> <http://www.w3.org/2000/01/rdf-schema#label> "Convert text to  date" .
<http://w3id.org/abdn/socialmedia/prism#toDate> <http://www.w3.org/1999/02/22-rdf-syntax-ns#type> <http://w3id.org/abdn/socialmedia/prism#DataPreparationMethod> .
<http://w3id.org/abdn/socialmedia/prism#collapseConsecutiveWhitespace> <http://www.w3.org/2000/01/rdf-schema#comment> "Data preparation method in which multiple whitespace characters are reduced to a single character.   Based on transformation of the same label in OpenRefine."@en .
<http://w3id.org/abdn/socialmedia/prism#collapseConsecutiveWhitespace> <http://www.w3.org/2004/02/skos/core#prefLabel> "Collapse consecutive whitespace" .
<http://w3id.org/abdn/socialmedia/prism#collapseConsecutiveWhitespace> <http://www.w3.org/2000/01/rdf-schema#label> "Collapse consecutive whitespace" .
<http://w3id.org/abdn/socialmedia/prism#collapseConsecutiveWhitespace> <http://www.w3.org/1999/02/22-rdf-syntax-ns#type> <http://w3id.org/abdn/socialmedia/prism#DataPreparationMethod> .
<http://w3id.org/abdn/socialmedia/prism#usedDataFrom> <http://www.w3.org/1999/02/22-rdf-syntax-ns#type> <http://www.w3.org/2002/07/owl#ObjectProperty> .
_:AX2dX2fe0ec5fX3aX158de32f70eX3aXX2dX7ffa <http://www.w3.org/2002/07/owl#allValuesFrom> <http://w3id.org/abdn/socialmedia/prism#DataPreparationActivity> .
_:AX2dX2fe0ec5fX3aX158de32f70eX3aXX2dX7ffa <http://www.w3.org/2002/07/owl#onProperty> <http://w3id.org/abdn/socialmedia/prism#usedDataFrom> .
_:AX2dX2fe0ec5fX3aX158de32f70eX3aXX2dX7ffa <http://www.w3.org/1999/02/22-rdf-syntax-ns#type> <http://www.w3.org/2002/07/owl#Restriction> .
<http://w3id.org/abdn/socialmedia/prism#toLowercase> <http://www.w3.org/2000/01/rdf-schema#comment> "Data preparation method in which text is converted to lowercase.   Based on transformation of the same label in OpenRefine."@en .
<http://w3id.org/abdn/socialmedia/prism#toLowercase> <http://www.w3.org/2004/02/skos/core#prefLabel> "Convert text to lowercase" .
<http://w3id.org/abdn/socialmedia/prism#toLowercase> <http://www.w3.org/2000/01/rdf-schema#label> "Convert text to lowercase" .
<http://w3id.org/abdn/socialmedia/prism#toLowercase> <http://www.w3.org/1999/02/22-rdf-syntax-ns#type> <http://w3id.org/abdn/socialmedia/prism#DataPreparationMethod> .
<http://w3id.org/abdn/socialmedia/prism#DataPreparationMethod> <http://www.w3.org/2000/01/rdf-schema#comment> "A method/technique used to prepare data in some way for analysis."@en .
<http://w3id.org/abdn/socialmedia/prism#DataPreparationMethod> <http://www.w3.org/2000/01/rdf-schema#label> "Data Preparation Method" .
<http://w3id.org/abdn/socialmedia/prism#DataPreparationMethod> <http://www.w3.org/1999/02/22-rdf-syntax-ns#type> <http://www.w3.org/2002/07/owl#Class> .
_:AX2dX2fe0ec5fX3aX158de32f70eX3aXX2dX7ff6 <http://www.w3.org/2002/07/owl#allValuesFrom> <http://w3id.org/abdn/socialmedia/prism#DataPreparationMethod> .
_:AX2dX2fe0ec5fX3aX158de32f70eX3aXX2dX7ff6 <http://www.w3.org/2002/07/owl#onProperty> <http://w3id.org/abdn/socialmedia/prism#preparationMethodUsed> .
_:AX2dX2fe0ec5fX3aX158de32f70eX3aXX2dX7ff6 <http://www.w3.org/1999/02/22-rdf-syntax-ns#type> <http://www.w3.org/2002/07/owl#Restriction> .
<http://w3id.org/abdn/socialmedia/prism#DataCollectionActivity> <http://www.w3.org/2000/01/rdf-schema#comment> "The activity of collecting data."@en .
<http://w3id.org/abdn/socialmedia/prism#DataCollectionActivity> <http://www.w3.org/2000/01/rdf-schema#label> "Data Collection Activity" .
<http://w3id.org/abdn/socialmedia/prism#DataCollectionActivity> <http://www.w3.org/2000/01/rdf-schema#subClassOf> _:AX2dX2fe0ec5fX3aX158de32f70eX3aXX2dX7ff8 .
<http://w3id.org/abdn/socialmedia/prism#DataCollectionActivity> <http://www.w3.org/2000/01/rdf-schema#subClassOf> _:AX2dX2fe0ec5fX3aX158de32f70eX3aXX2dX7ff9 .
<http://w3id.org/abdn/socialmedia/prism#DataCollectionActivity> <http://www.w3.org/1999/02/22-rdf-syntax-ns#type> <http://www.w3.org/2002/07/owl#Class> .
<http://w3id.org/abdn/socialmedia/prism#toText> <http://www.w3.org/2000/01/rdf-schema#comment> "Data preparation method in which the type of a datum is changed to text.   Based on transformation of the same name in OpenRefine."@en .
<http://w3id.org/abdn/socialmedia/prism#toText> <http://www.w3.org/2004/02/skos/core#prefLabel> "Convert to text" .
<http://w3id.org/abdn/socialmedia/prism#toText> <http://www.w3.org/2000/01/rdf-schema#label> "Convert to text" .
<http://w3id.org/abdn/socialmedia/prism#toText> <http://www.w3.org/1999/02/22-rdf-syntax-ns#type> <http://w3id.org/abdn/socialmedia/prism#DataPreparationMethod> .
<http://w3id.org/abdn/socialmedia/prism#toUppercase> <http://www.w3.org/2000/01/rdf-schema#comment> "Data preparation method in which text is converted to uppercase.   Based on transformation of the same label in OpenRefine."@en .
<http://w3id.org/abdn/socialmedia/prism#toUppercase> <http://www.w3.org/2004/02/skos/core#prefLabel> "Convert text to uppercase" .
<http://w3id.org/abdn/socialmedia/prism#toUppercase> <http://www.w3.org/2000/01/rdf-schema#label> "Convert text to uppercase" .
<http://w3id.org/abdn/socialmedia/prism#toUppercase> <http://www.w3.org/1999/02/22-rdf-syntax-ns#type> <http://w3id.org/abdn/socialmedia/prism#DataPreparationMethod> .
<http://w3id.org/abdn/socialmedia/prism#dataCollectionEnded> <http://www.w3.org/2000/01/rdf-schema#comment> "The date that the activity of collected data ended."@en .
<http://w3id.org/abdn/socialmedia/prism#dataCollectionEnded> <http://www.w3.org/2000/01/rdf-schema#label> "data Collection Ended" .
<http://w3id.org/abdn/socialmedia/prism#dataCollectionEnded> <http://www.w3.org/2000/01/rdf-schema#range> <http://www.w3.org/2001/XMLSchema#date> .
<http://w3id.org/abdn/socialmedia/prism#dataCollectionEnded> <http://www.w3.org/1999/02/22-rdf-syntax-ns#type> <http://www.w3.org/2002/07/owl#DatatypeProperty> .
<http://w3id.org/abdn/socialmedia/prism#filterData> <http://www.w3.org/2000/01/rdf-schema#comment> "Data preparation method in which a subset of a a dataset is created based on filtering data in the original."@en .
<http://w3id.org/abdn/socialmedia/prism#filterData> <http://www.w3.org/2004/02/skos/core#prefLabel> "Filter data" .
<http://w3id.org/abdn/socialmedia/prism#filterData> <http://www.w3.org/2000/01/rdf-schema#label> "Filter data" .
<http://w3id.org/abdn/socialmedia/prism#filterData> <http://www.w3.org/1999/02/22-rdf-syntax-ns#type> <http://w3id.org/abdn/socialmedia/prism#DataPreparationMethod> .
<http://w3id.org/abdn/socialmedia/prism#toTitlecase> <http://www.w3.org/2000/01/rdf-schema#comment> "Data preparation method in which text is converted to title case.   Based on transformation of the same label in OpenRefine."@en .
<http://w3id.org/abdn/socialmedia/prism#toTitlecase> <http://www.w3.org/2004/02/skos/core#prefLabel> "Convert text to titlecase" .
<http://w3id.org/abdn/socialmedia/prism#toTitlecase> <http://www.w3.org/2000/01/rdf-schema#label> "Convert text to titlecase" .
<http://w3id.org/abdn/socialmedia/prism#toTitlecase> <http://www.w3.org/1999/02/22-rdf-syntax-ns#type> <http://w3id.org/abdn/socialmedia/prism#DataPreparationMethod> .
<http://w3id.org/abdn/socialmedia/prism#collectedUsing> <http://www.w3.org/2000/01/rdf-schema#comment> "Relationship between a dataset and a tool that was used to collect the data."@en .
<http://w3id.org/abdn/socialmedia/prism#collectedUsing> <http://www.w3.org/2000/01/rdf-schema#label> "collected Using" .
<http://w3id.org/abdn/socialmedia/prism#collectedUsing> <http://www.w3.org/2000/01/rdf-schema#range> <http://w3id.org/abdn/socialmedia/prism#DataCollectionTool> .
<http://w3id.org/abdn/socialmedia/prism#collectedUsing> <http://www.w3.org/1999/02/22-rdf-syntax-ns#type> <http://www.w3.org/2002/07/owl#ObjectProperty> .
<http://w3id.org/abdn/socialmedia/prism#DataAnalysisMethod> <http://www.w3.org/2000/01/rdf-schema#comment> "A method utilised to analyse data."@en .
<http://w3id.org/abdn/socialmedia/prism#DataAnalysisMethod> <http://www.w3.org/2000/01/rdf-schema#label> "Data analysis method" .
<http://w3id.org/abdn/socialmedia/prism#DataAnalysisMethod> <http://www.w3.org/1999/02/22-rdf-syntax-ns#type> <http://www.w3.org/2002/07/owl#Class> .
<http://w3id.org/abdn/socialmedia/prism#unescapeHtmlEntities> <http://www.w3.org/2000/01/rdf-schema#comment> "Data preparation method in which escaped HTML characters (e.g. &amp;amp;) are unescaped (e..g back to &amp;).   Based on transformation of the same label in OpenRefine."@en .
<http://w3id.org/abdn/socialmedia/prism#unescapeHtmlEntities> <http://www.w3.org/2004/02/skos/core#prefLabel> "Unescape HTML entities" .
<http://w3id.org/abdn/socialmedia/prism#unescapeHtmlEntities> <http://www.w3.org/2000/01/rdf-schema#label> "Unescape HTML entities" .
<http://w3id.org/abdn/socialmedia/prism#unescapeHtmlEntities> <http://www.w3.org/1999/02/22-rdf-syntax-ns#type> <http://w3id.org/abdn/socialmedia/prism#DataPreparationMethod> .
<http://w3id.org/abdn/socialmedia/prism#DataAnalysisActivity> <http://www.w3.org/2000/01/rdf-schema#comment> "The activity of performing some form of data analysis"@en .
<http://w3id.org/abdn/socialmedia/prism#DataAnalysisActivity> <http://www.w3.org/2000/01/rdf-schema#label> "Data analysis activity" .
<http://w3id.org/abdn/socialmedia/prism#DataAnalysisActivity> <http://www.w3.org/2000/01/rdf-schema#subClassOf> _:AX2dX2fe0ec5fX3aX158de32f70eX3aXX2dX7ffa .
<http://w3id.org/abdn/socialmedia/prism#DataAnalysisActivity> <http://www.w3.org/2000/01/rdf-schema#subClassOf> _:AX2dX2fe0ec5fX3aX158de32f70eX3aXX2dX7ffb .
<http://w3id.org/abdn/socialmedia/prism#DataAnalysisActivity> <http://www.w3.org/2000/01/rdf-schema#subClassOf> _:AX2dX2fe0ec5fX3aX158de32f70eX3aXX2dX7ffc .
<http://w3id.org/abdn/socialmedia/prism#DataAnalysisActivity> <http://www.w3.org/1999/02/22-rdf-syntax-ns#type> <http://www.w3.org/2002/07/owl#Class> .
<http://w3id.org/abdn/socialmedia/prism#analysisMethodUsed> <http://www.w3.org/2000/01/rdf-schema#comment> "Relationship between a data analysis activity and the analysis method used."@en .
<http://w3id.org/abdn/socialmedia/prism#analysisMethodUsed> <http://www.w3.org/2000/01/rdf-schema#label> "analysis method used" .
<http://w3id.org/abdn/socialmedia/prism#analysisMethodUsed> <http://www.w3.org/1999/02/22-rdf-syntax-ns#type> <http://www.w3.org/2002/07/owl#ObjectProperty> .
<http://w3id.org/abdn/socialmedia/prism#DataPreparationActivity> <http://www.w3.org/2000/01/rdf-schema#comment> "The activity of preparing data, typically before or in-order-to perform some analysis."@en .
<http://w3id.org/abdn/socialmedia/prism#DataPreparationActivity> <http://www.w3.org/2000/01/rdf-schema#label> "Data Preparation Activity" .
<http://w3id.org/abdn/socialmedia/prism#DataPreparationActivity> <http://www.w3.org/2000/01/rdf-schema#subClassOf> _:AX2dX2fe0ec5fX3aX158de32f70eX3aXX2dX7ff6 .
<http://w3id.org/abdn/socialmedia/prism#DataPreparationActivity> <http://www.w3.org/2000/01/rdf-schema#subClassOf> _:AX2dX2fe0ec5fX3aX158de32f70eX3aXX2dX7ff7 .
<http://w3id.org/abdn/socialmedia/prism#DataPreparationActivity> <http://www.w3.org/1999/02/22-rdf-syntax-ns#type> <http://www.w3.org/2002/07/owl#Class> .
_:AX2dX2fe0ec5fX3aX158de32f70eX3aXX2dX7ff9 <http://www.w3.org/2002/07/owl#onDataRange> <http://www.w3.org/2002/07/owl#rational> .
_:AX2dX2fe0ec5fX3aX158de32f70eX3aXX2dX7ff9 <http://www.w3.org/2002/07/owl#qualifiedCardinality> "1"^^<http://www.w3.org/2001/XMLSchema#nonNegativeInteger> .
_:AX2dX2fe0ec5fX3aX158de32f70eX3aXX2dX7ff9 <http://www.w3.org/2002/07/owl#onProperty> <http://w3id.org/abdn/socialmedia/prism#dataCollectionEnded> .
_:AX2dX2fe0ec5fX3aX158de32f70eX3aXX2dX7ff9 <http://www.w3.org/1999/02/22-rdf-syntax-ns#type> <http://www.w3.org/2002/07/owl#Restriction> .
<http://w3id.org/abdn/socialmedia/prism#collectedFromService> <http://www.w3.org/2000/01/rdf-schema#comment> "Relationship between a dataset and a service/website that the data was collected from."@en .
<http://w3id.org/abdn/socialmedia/prism#collectedFromService> <http://www.w3.org/2000/01/rdf-schema#label> "collected From Service" .
<http://w3id.org/abdn/socialmedia/prism#collectedFromService> <http://www.w3.org/1999/02/22-rdf-syntax-ns#type> <http://www.w3.org/2002/07/owl#DatatypeProperty> .
<http://w3id.org/abdn/socialmedia/prism#> <http://www.w3.org/1999/02/22-rdf-syntax-ns#type> <http://www.w3.org/2002/07/owl#Ontology> .
<http://w3id.org/abdn/socialmedia/prism#> <http://purl.org/dc/elements/1.1/creator> "David Corsar"^^<http://www.w3.org/2001/XMLSchema#string> .
<http://w3id.org/abdn/socialmedia/prism#> <http://purl.org/dc/elements/1.1/title> "The Provenance of Research Involving Social Media ontology"^^<http://www.w3.org/2001/XMLSchema#string> .
<http://w3id.org/abdn/socialmedia/prism#> <http://www.w3.org/2002/07/owl#versionInfo> "Revision: 0.1"^^<http://www.w3.org/2001/XMLSchema#string> .
<http://w3id.org/abdn/socialmedia/prism#> <http://purl.org/dc/elements/1.1/description> "This ontology is designed to capture provenance meta-data describing the use of social media data in research projects."@en .
<http://w3id.org/abdn/socialmedia/prism#> <http://purl.org/dc/elements/1.1/creator> "Milan Markovic"^^<http://www.w3.org/2001/XMLSchema#string> .
<http://w3id.org/abdn/socialmedia/prism#> <http://www.w3.org/2000/01/rdf-schema#label> "The Provenance of Research Involving Social Media ontology" .
<http://w3id.org/abdn/socialmedia/prism#> <http://web.resource.org/cc/license> <https://creativecommons.org/licenses/by/4.0/> .
<http://w3id.org/abdn/socialmedia/prism#> <http://purl.org/dc/elements/1.1/rights> "Copyright \u00A9 2015 University of Aberdeen"^^<http://www.w3.org/2001/XMLSchema#string> .
<http://w3id.org/abdn/socialmedia/prism#> <http://www.w3.org/2000/01/rdf-schema#comment> "This ontology is designed to capture provenance meta-data describing the use of social media data in research projects."@en .
_:AX2dX2fe0ec5fX3aX158de32f70eX3aXX2dX7ffc <http://www.w3.org/2002/07/owl#allValuesFrom> <http://dbpedia.org/resource/dataset> .
_:AX2dX2fe0ec5fX3aX158de32f70eX3aXX2dX7ffc <http://www.w3.org/2002/07/owl#onProperty> <http://www.w3.org/ns/prov#used> .
_:AX2dX2fe0ec5fX3aX158de32f70eX3aXX2dX7ffc <http://www.w3.org/1999/02/22-rdf-syntax-ns#type> <http://www.w3.org/2002/07/owl#Restriction> .
<http://w3id.org/abdn/socialmedia/prism#removeData> <http://www.w3.org/2000/01/rdf-schema#comment> "Data preparation method in which data is removed from a dataset."@en .
<http://w3id.org/abdn/socialmedia/prism#removeData> <http://www.w3.org/2004/02/skos/core#prefLabel> "Remove data" .
<http://w3id.org/abdn/socialmedia/prism#removeData> <http://www.w3.org/2000/01/rdf-schema#label> "Remove data" .
<http://w3id.org/abdn/socialmedia/prism#removeData> <http://www.w3.org/1999/02/22-rdf-syntax-ns#type> <http://w3id.org/abdn/socialmedia/prism#DataPreparationMethod> .
<http://w3id.org/abdn/socialmedia/prism#trimLeadingTrailingWhitespace> <http://www.w3.org/2000/01/rdf-schema#comment> "Data preparation method in which leading and trailing whitespace are removed from a piece of text.  Based on transformation of the same label in OpenRefine."@en .
<http://w3id.org/abdn/socialmedia/prism#trimLeadingTrailingWhitespace> <http://www.w3.org/2004/02/skos/core#prefLabel> "Trim leading and trailing whitespace" .
<http://w3id.org/abdn/socialmedia/prism#trimLeadingTrailingWhitespace> <http://www.w3.org/2000/01/rdf-schema#label> "Trim leading and trailing whitespace" .
<http://w3id.org/abdn/socialmedia/prism#trimLeadingTrailingWhitespace> <http://www.w3.org/1999/02/22-rdf-syntax-ns#type> <http://w3id.org/abdn/socialmedia/prism#DataPreparationMethod> .
